\let\negmedspace\undefined
\let\negthickspace\undefined
\documentclass[journal,12pt,twocolumn]{IEEEtran}
\usepackage{cite}
\usepackage{amsmath,amssymb,amsfonts,amsthm}
\usepackage{algorithmic}
\usepackage{graphicx}
\usepackage{textcomp}
\usepackage{xcolor}
\usepackage{txfonts}
\usepackage{listings}
\usepackage{enumitem}
\usepackage{mathtools}
\usepackage{gensymb}
\usepackage{comment}
\usepackage[breaklinks=true]{hyperref}
\usepackage{tkz-euclide} 
\usepackage{listings}
\usepackage{gvv}                                        
\def\inputGnumericTable{}                                 
\usepackage[latin1]{inputenc}                                
\usepackage{color}                                            
\usepackage{array}                                            
\usepackage{longtable}                                       
\usepackage{calc}                                             
\usepackage{multirow}                                         
\usepackage{hhline}                                           
\usepackage{ifthen}                                           
\usepackage{lscape}
\usepackage{caption}

\newtheorem{theorem}{Theorem}[section]
\newtheorem{problem}{Problem}
\newtheorem{proposition}{Proposition}[section]
\newtheorem{lemma}{Lemma}[section]
\newtheorem{corollary}[theorem]{Corollary}
\newtheorem{example}{Example}[section]
\newtheorem{definition}[problem]{Definition}
\newcommand{\BEQA}{\begin{eqnarray}}
\newcommand{\EEQA}{\end{eqnarray}}
\newcommand{\define}{\stackrel{\triangle}{=}}
\theoremstyle{remark}
\newtheorem{rem}{Remark}
\begin{document}

\bibliographystyle{IEEEtran}
\vspace{3cm}

\title{10.5.4}
\author{EE23BTECH11029 - Kanishk}
\maketitle
\newpage

\bigskip

\renewcommand{\thefigure}{\theenumi}
\renewcommand{\thetable}{\theenumi}
\textbf{Question}:\\
The houses of a row are numbered consecutively from 1 to 49. Show that there is a value
of x such that the sum of the numbers of the houses preceding the house numbered is equal to the sum of the numbers of the houses following it. Find this value of x.\\
Hint:$ S_{x-1}=S_{49}-S_x$

\textbf{Solution}:\\

\begin{table}[ht]
    \centering
    \def\arraystretch{1.5}
    \input{tables/TABLE1.tex}
   \caption{Input Parameters}
   \label{tab:10.5.4}
\end{table}


For an AP:
\begin{align}
X\brak{z}&=\frac{x\brak{0}}{1-z^{-1}}+ \frac{dz^{-1}}{\brak{1-z^{-1}}^{2}}\\
\implies X\brak{z}&=\frac{1}{1-z^{-1}}+ \frac{z^{-1}}{\brak{1-z^{-1}}^{2}}\\
&=\frac{1}{\brak{1-z^{-1}}^{2}},\quad \abs{z} > 1
\end{align}

\begin{align}
y\brak{n}&=x\brak{n}*u\brak{n}\\
\implies y\brak{Z}&=X\brak{z}*U\brak{z}\\
Y\brak{z}&= \frac{1}{\brak{1-z^{-1}}^{3}},\quad \abs{z}>1
\end{align}
Contour Integration to find inverse of Z-transform,

\begin{align}
y\brak{n}&=\frac{1}{2\pi j}\oint_c Y\brak{z}z^{n-1} \,dz\\
&=\frac{1}{2\pi j} \oint_c \frac{1}{\brak{1-z^{-1}}^{3}}z^{n-1} \,dz
\end{align}
We can observe that Pole is repeated 3 times thus m=3,
\begin{align}
R&=\frac{1}{\brak {m-1}!}\lim\limits_{z\to a}\frac{d^{m-1}}{dz^{m-1}}\brak {{(z-a)}^{m}f\brak z}  \\
&=\frac{1}{\brak {2}!}\lim\limits_{z\to 1}\frac{d^{2}}{dz^{2}}\brak {{(z-1)}^{3}\frac{z^{n+2}}{{(z-1)}^3}}\\
&=\frac{1}{\brak {2}!}\lim\limits_{z\to 1}\frac{d^{2}}{dz^{2}}\brak{z^{n+2}}\\
&=\frac{n+1}{2}\brak{n+2}
\end{align}

\begin{align}
    \therefore y\brak{n}=\frac{n+1}{2}\brak{n+2}
\end{align}

\begin{align}
y\brak{x-2}&=y\brak{48}-y\brak{x-1}\\
From \tabref{tab:10.5.4}:\\
\frac{x-1}{2}\brak{x}&=\frac{49}{2}\brak{50}-\frac{x}{2}\brak{x+1}\\
\brak{x-1}&=49\times50 - x\brak{x+1}\\
2x^{2}&=49\times50\\
x^{2}&=49\times50\\
x&=35
\end{align}


\begin{figure}[h]
    
    \includegraphics[width=\columnwidth]{figs/fig1.png}
    \caption{Plot y(n) vs n}
\end{figure}

 \end{document}